frodo/code/Hacl.Frodo.Random.fsti
@@ -7,17 +7,25 @@ open LowStar.Buffer
 open Lib.IntTypes
 open Lib.PQ.Buffer
 
+module S = Spec.Frodo.Random
+
+val state: b:buffer uint8{ recallable b }
+
 val randombytes_init_:
     entropy_input:lbuffer uint8 48
   -> Stack unit
-    (requires fun h -> live h entropy_input)
-    (ensures  fun h0 _ h1 -> live h1 entropy_input)
+    (requires fun h -> live h entropy_input /\ live h state)
+    (ensures  fun h0 _ h1 -> 
+      modifies (loc_buffer state) h0 h1 /\
+      as_seq h1 state == S.randombytes_init_ (as_seq h0 entropy_input))
 
 val randombytes_:
     len:size_t
   -> res:lbuffer uint8 (v len)
   -> Stack unit
-    (requires fun h -> live h res)
+    (requires fun h -> live h res /\ live h state)
     (ensures  fun h0 _ h1 ->
-      modifies (loc_buffer res) h0 h1 /\
-      as_seq h1 res == Spec.Frodo.Random.randombytes_ (v len))
+      modifies (loc_union (loc_buffer res) (loc_buffer state)) h0 h1 /\
+      as_seq h1 res == fst (S.randombytes_ (as_seq h0 state) (v len)) /\
+      as_seq h1 state == snd (S.randombytes_ (as_seq h0 state) (v len)))
+
